Use better naming

DSL/Array.v
@@ -10,29 +10,29 @@ Definition sigArray := list sig.
 
 Module Get.
 
-  Inductive get : sigArray -> sig -> nat -> Prop :=
-  | get_frst: forall ss s, get (s :: ss) s 0
-  | get_step: forall ss s s' i, get ss s i -> get (s' :: ss) s (S i).
+  Inductive iget : sigArray -> sig -> nat -> Prop :=
+  | iget_frst: forall ss s, iget (s :: ss) s 0
+  | iget_step: forall ss s s' i, iget ss s i -> iget (s' :: ss) s (S i).
 
-  Fixpoint fget (ss : sigArray) (s : sig) (i : nat) : Prop :=
+  Fixpoint get (ss : sigArray) (s : sig) (i : nat) : Prop :=
     match ss, i with
     | nil, _ => False
     | s' :: _, O => s' = s
-    | _ :: ss', S i' => fget ss' s i'
+    | _ :: ss', S i' => get ss' s i'
     end.
 
 End Get.
 
 Module Init.
 
-  Inductive init : sigArray -> sig -> nat -> Prop :=
-  | init_zero: forall s, init nil s 0
-  | init_succ: forall ss s i, init ss s i -> init (s :: ss) s (S i).
+  Inductive iinit : sigArray -> sig -> nat -> Prop :=
+  | iinit_zero: forall s, iinit nil s 0
+  | iinit_succ: forall ss s i, iinit ss s i -> iinit (s :: ss) s (S i).
 
-  Fixpoint finit (ss : sigArray) (s : sig) (n : nat) : Prop :=
+  Fixpoint init (ss : sigArray) (s : sig) (n : nat) : Prop :=
     match ss, n with
     | nil, O => True
-    | s' :: ss', S n' => s' = s /\ finit ss' s n'
+    | s' :: ss', S n' => s' = s /\ init ss' s n'
     | _, _ => False
     end.
 
@@ -40,14 +40,14 @@ End Init.
 
 Module Scale.
 
-  Inductive scale : sig -> sigArray -> sigArray -> Prop :=
-  | scale_nil: forall c, scale c nil nil
-  | scale_cons: forall c ss ss' s, scale c ss ss' -> scale c (s :: ss) (F.mul c s :: ss').
+  Inductive iscale : sig -> sigArray -> sigArray -> Prop :=
+  | iscale_nil: forall c, iscale c nil nil
+  | iscale_cons: forall c ss ss' s, iscale c ss ss' -> iscale c (s :: ss) (F.mul c s :: ss').
 
-  Fixpoint fscale (c : sig) (s1 s2 : sigArray) : Prop :=
+  Fixpoint scale (c : sig) (s1 s2 : sigArray) : Prop :=
     match s1, s2 with
     | nil, nil => True
-    | s' :: s1', s'' :: s2' => s'' = F.mul c s' /\ fscale c s1' s2'
+    | s' :: s1', s'' :: s2' => s'' = F.mul c s' /\ scale c s1' s2'
     | _, _ => False
     end.
 
@@ -55,39 +55,39 @@ End Scale.
 
 Module Sum.
 
-  Inductive sum : sigArray -> sig -> Prop :=
-  | sum_nil: sum nil F.zero
-  | sum_cons: forall ss s s', sum ss s -> sum (s' :: ss) (F.add s' s).
+  Inductive isum : sigArray -> sig -> Prop :=
+  | isum_nil: isum nil F.zero
+  | isum_cons: forall ss s s', isum ss s -> isum (s' :: ss) (F.add s' s).
 
-  Fixpoint fsum (ss : sigArray) (s : sig) : Prop :=
+  Fixpoint sum (ss : sigArray) (s : sig) : Prop :=
     match ss with
     | nil => s = F.zero
-    | s' :: ss' => fsum ss' (F.sub s s')
+    | s' :: ss' => sum ss' (F.sub s s')
     end.
 
 End Sum.
 
 Module Map.
 
-  Inductive map {A : Type} : (sig -> A) -> sigArray -> list A -> Prop :=
-  | map_nil: forall f, map f nil nil
-  | map_cons: forall f ss a s, map f ss a -> map f (s :: ss) (f s :: a).
+  Inductive imap {A : Type} : (sig -> A) -> sigArray -> list A -> Prop :=
+  | imap_nil: forall f, imap f nil nil
+  | imap_cons: forall f ss a s, imap f ss a -> imap f (s :: ss) (f s :: a).
 
-  Fixpoint fmap {A : Type} (f : sig -> A) (ss : sigArray) (l : list A) : Prop :=
+  Fixpoint map {A : Type} (f : sig -> A) (ss : sigArray) (l : list A) : Prop :=
     match ss, l with
     | nil, nil => True
-    | s' :: ss', a :: l' => a = f s' /\ fmap f ss' l'
+    | s' :: ss', a :: l' => a = f s' /\ map f ss' l'
     | _, _ => False
     end.
 
-  Lemma fmap_sound: forall A (f : sig -> A) ss l, fmap f ss l -> List.map f ss = l.
+  Lemma map_sound: forall A (f : sig -> A) ss l, map f ss l -> List.map f ss = l.
   Proof.
     intros A f.
     induction ss; intros; simpl in H; simpl; destruct l; intuition.
     - apply IHss in H1. rewrite <- H0, H1. reflexivity.
   Qed.
 
-  Lemma fmap_complete: forall A (f : sig -> A) ss, fmap f ss (List.map f ss).
+  Lemma map_complete: forall A (f : sig -> A) ss, map f ss (List.map f ss).
   Proof.
     intros A f. induction ss; simpl; auto.
   Qed.
@@ -96,78 +96,78 @@ End Map.
 
 Module Fold.
 
-  Inductive foldl {A : Type} : (A -> sig -> A) -> sigArray -> A -> A -> Prop :=
-  | foldl_nil: forall f a, foldl f nil a a
-  | foldl_app: forall f ss a a' s, foldl f ss a a' -> foldl f (ss ++ (cons s nil)) a (f a' s).
+  Inductive ifoldl {A : Type} : (A -> sig -> A) -> sigArray -> A -> A -> Prop :=
+  | ifoldl_nil: forall f a, ifoldl f nil a a
+  | ifoldl_app: forall f ss a a' s, ifoldl f ss a a' -> ifoldl f (ss ++ (cons s nil)) a (f a' s).
 
-  Fixpoint ffoldl {A : Type} (f : A -> sig -> A) (ss : sigArray) (acc a : A) : Prop :=
+  Fixpoint foldl {A : Type} (f : A -> sig -> A) (ss : sigArray) (acc a : A) : Prop :=
     match ss with
     | nil => a = acc
     | s' :: ss' =>
         let acc' := f acc s' in
-        ffoldl f ss' acc' a
+        foldl f ss' acc' a
     end.
 
-  Lemma ffoldl_sound: forall A (f : A -> sig -> A) ss acc a,
-      ffoldl f ss acc a -> fold_left f ss acc = a.
+  Lemma foldl_sound: forall A (f : A -> sig -> A) ss acc a,
+      foldl f ss acc a -> fold_left f ss acc = a.
   Proof.
     intros A f. induction ss; intros; simpl in H; simpl; auto.
   Qed.
 
-  Lemma ffoldl_complete: forall A (f : A -> sig -> A) ss acc,
-      ffoldl f ss acc (fold_left f ss acc).
+  Lemma foldl_complete: forall A (f : A -> sig -> A) ss acc,
+      foldl f ss acc (fold_left f ss acc).
   Proof.
     intros A f. induction ss; intros; simpl; auto.
   Qed.
 
-  Inductive foldr {A : Type} : (sig -> A -> A) -> A -> sigArray -> A -> Prop :=
-  | foldr_nil: forall f a, foldr f a nil a
-  | foldr_cons: forall f ss a a' s, foldr f a ss a' -> foldr f a (s :: ss) (f s a').
+  Inductive ifoldr {A : Type} : (sig -> A -> A) -> A -> sigArray -> A -> Prop :=
+  | ifoldr_nil: forall f a, ifoldr f a nil a
+  | ifoldr_cons: forall f ss a a' s, ifoldr f a ss a' -> ifoldr f a (s :: ss) (f s a').
 
-  Definition ffoldr {A : Type} (f : sig -> A -> A) (acc : A) (ss : sigArray) (a : A) : Prop :=
-    ffoldl (fun acc s => f s acc) (rev ss) acc a.
+  Definition foldr {A : Type} (f : sig -> A -> A) (acc : A) (ss : sigArray) (a : A) : Prop :=
+    foldl (fun acc s => f s acc) (rev ss) acc a.
 
-  Lemma ffoldr_sound: forall A (f : sig -> A -> A) acc ss a,
-      ffoldr f acc ss a -> fold_right f acc ss = a.
+  Lemma foldr_sound: forall A (f : sig -> A -> A) acc ss a,
+      foldr f acc ss a -> fold_right f acc ss = a.
   Proof.
     intros A f acc ss. revert acc.
-    induction ss; intros; unfold ffoldr in H; simpl in H; simpl.
+    induction ss; intros; unfold foldr in H; simpl in H; simpl.
     - auto.
-    - apply ffoldl_sound in H. rewrite fold_left_app in H. simpl in H.
-      assert (H0: ffoldl (fun (acc : A) (s : sig) => f s acc) (rev ss) acc
+    - apply foldl_sound in H. rewrite fold_left_app in H. simpl in H.
+      assert (H0: foldl (fun (acc : A) (s : sig) => f s acc) (rev ss) acc
                     (fold_left (fun (acc : A) (s : sig) => f s acc) (rev ss) acc)).
-      { apply ffoldl_complete. }
-      unfold ffoldr in IHss. apply IHss in H0. rewrite <- H0 in H. apply H.
+      { apply foldl_complete. }
+      unfold foldr in IHss. apply IHss in H0. rewrite <- H0 in H. apply H.
   Qed.
 
-  Lemma ffoldr_complete: forall A (f : sig -> A -> A) acc ss,
-      ffoldr f acc ss (fold_right f acc ss).
+  Lemma foldr_complete: forall A (f : sig -> A -> A) acc ss,
+      foldr f acc ss (fold_right f acc ss).
   Proof.
     intros A f acc ss. revert acc.
-    induction ss; intros; unfold ffoldr; simpl.
+    induction ss; intros; unfold foldr; simpl.
     - auto.
     - assert (H0: fold_left (fun (acc0 : A) (s : sig) => f s acc0)
                     (rev ss ++ a :: nil) acc = (f a (fold_right f acc ss))).
-      { rewrite fold_left_app. simpl. unfold ffoldr in IHss.
+      { rewrite fold_left_app. simpl. unfold foldr in IHss.
         specialize IHss with (acc := acc) as H0'.
-        apply ffoldl_sound in H0'. rewrite H0'. reflexivity. }
-      rewrite <- H0. apply ffoldl_complete.
+        apply foldl_sound in H0'. rewrite H0'. reflexivity. }
+      rewrite <- H0. apply foldl_complete.
   Qed.
 
 End Fold.
 
 Module Map2.
 
-  Inductive map2 {A : Type} : (sig -> sig -> A) -> sigArray -> sigArray -> list A -> Prop :=
-  | map2_nil_l: forall f ss, map2 f nil ss nil
-  | map2_nil_r: forall f ss, map2 f ss nil nil
-  | map2_cons: forall f ss1 ss2 a s1 s2, map2 f ss1 ss2 a -> map2 f (s1 :: ss1) (s2 :: ss2) (f s1 s2 :: a).
+  Inductive imap2 {A : Type} : (sig -> sig -> A) -> sigArray -> sigArray -> list A -> Prop :=
+  | imap2_nil_l: forall f ss, imap2 f nil ss nil
+  | imap2_nil_r: forall f ss, imap2 f ss nil nil
+  | imap2_cons: forall f ss1 ss2 a s1 s2, imap2 f ss1 ss2 a -> imap2 f (s1 :: ss1) (s2 :: ss2) (f s1 s2 :: a).
 
-  Fixpoint fmap2 {A : Type} (f : sig -> sig -> A) (s1 s2 : sigArray) (l : list A) : Prop :=
+  Fixpoint map2 {A : Type} (f : sig -> sig -> A) (s1 s2 : sigArray) (l : list A) : Prop :=
     match s1, s2, l with
     | nil, nil, nil => True
     | s' :: s1', s'' :: s2', a :: l' =>
-        a = f s' s'' /\ fmap2 f s1' s2' l'
+        a = f s' s'' /\ map2 f s1' s2' l'
     | _, _, _ => False
     end.
 
@@ -175,51 +175,51 @@ End Map2.
 
 Module Fold2.
 
-  Inductive foldl2 {A : Type} : (A -> sig -> sig -> A) -> sigArray -> sigArray -> A -> A -> Prop :=
-  | foldl2_nil_l: forall f ss a, foldl2 f nil ss a a
-  | foldl2_nil_r: forall f ss a, foldl2 f ss nil a a
-  | foldl2_app: forall f ss1 ss2 a a' s1 s2,
-      foldl2 f ss1 ss2 a a' -> foldl2 f (ss1 ++ (cons s1 nil)) (ss2 ++ (cons s2 nil)) a (f a' s1 s2).
+  Inductive ifoldl2 {A : Type} : (A -> sig -> sig -> A) -> sigArray -> sigArray -> A -> A -> Prop :=
+  | ifoldl2_nil_l: forall f ss a, ifoldl2 f nil ss a a
+  | ifoldl2_nil_r: forall f ss a, ifoldl2 f ss nil a a
+  | ifoldl2_app: forall f ss1 ss2 a a' s1 s2,
+      ifoldl2 f ss1 ss2 a a' -> ifoldl2 f (ss1 ++ (cons s1 nil)) (ss2 ++ (cons s2 nil)) a (f a' s1 s2).
 
-  Fixpoint ffoldl2 {A : Type} (f : A -> sig -> sig -> A) (s1 s2 : sigArray) (acc a : A) : Prop :=
+  Fixpoint foldl2 {A : Type} (f : A -> sig -> sig -> A) (s1 s2 : sigArray) (acc a : A) : Prop :=
     match s1, s2 with
     | nil, nil => a = acc
     | s' :: s1', s'' :: s2' =>
         let acc' := f acc s' s'' in
-        ffoldl2 f s1' s2' acc' a
+        foldl2 f s1' s2' acc' a
     | _, _ => False
     end.
 
-  Inductive foldr2 {A : Type} : (sig -> sig -> A -> A) -> A -> sigArray -> sigArray -> A -> Prop :=
-  | foldr2_nil_l: forall f ss a, foldr2 f a nil ss a
-  | foldr2_nil_r: forall f ss a, foldr2 f a ss nil a
-  | foldr2_cons: forall f ss1 ss2 a a' s1 s2,
-      foldr2 f a ss1 ss2 a' -> foldr2 f a (s1 :: ss1) (s2 :: ss2) (f s1 s2 a').
+  Inductive ifoldr2 {A : Type} : (sig -> sig -> A -> A) -> A -> sigArray -> sigArray -> A -> Prop :=
+  | ifoldr2_nil_l: forall f ss a, ifoldr2 f a nil ss a
+  | ifoldr2_nil_r: forall f ss a, ifoldr2 f a ss nil a
+  | ifoldr2_cons: forall f ss1 ss2 a a' s1 s2,
+      ifoldr2 f a ss1 ss2 a' -> ifoldr2 f a (s1 :: ss1) (s2 :: ss2) (f s1 s2 a').
 
-  Definition ffoldr2 {A : Type} (f : sig -> sig -> A -> A) (acc : A) (s1 s2 : sigArray) (a : A) : Prop :=
-    ffoldl2 (fun acc s' s'' => f s' s'' acc) (rev s1) (rev s2) acc a.
+  Definition foldr2 {A : Type} (f : sig -> sig -> A -> A) (acc : A) (s1 s2 : sigArray) (a : A) : Prop :=
+    foldl2 (fun acc s' s'' => f s' s'' acc) (rev s1) (rev s2) acc a.
 
 End Fold2.
 
 Module Elem.
 
+  Definition ielem_add := Map2.imap2 F.add.
+  Definition ielem_sub := Map2.imap2 F.sub.
+  Definition ielem_mul := Map2.imap2 F.mul.
+
   Definition elem_add := Map2.map2 F.add.
   Definition elem_sub := Map2.map2 F.sub.
   Definition elem_mul := Map2.map2 F.mul.
 
-  Definition felem_add := Map2.fmap2 F.add.
-  Definition felem_sub := Map2.fmap2 F.sub.
-  Definition felem_mul := Map2.fmap2 F.mul.
+  Inductive ielem_eq : sigArray -> sigArray -> Prop :=
+  | ielem_eq_nil: ielem_eq nil nil
+  | ielem_eq_cons: forall s1 s2 s, ielem_eq s1 s2 -> ielem_eq (s :: s1) (s :: s2).
 
-  Inductive elem_eq : sigArray -> sigArray -> Prop :=
-  | elem_eq_nil: elem_eq nil nil
-  | elem_eq_cons: forall s1 s2 s, elem_eq s1 s2 -> elem_eq (s :: s1) (s :: s2).
-
-  Fixpoint felem_eq (s1 s2 : sigArray) : Prop :=
+  Fixpoint elem_eq (s1 s2 : sigArray) : Prop :=
     match s1, s2 with
     | nil, nil => True
     | s' :: s1', s'' :: s2' =>
-        s' = s'' /\ felem_eq s1' s2'
+        s' = s'' /\ elem_eq s1' s2'
     | _, _ => False
     end.
 
